Launchbury/ArityCorrect.thy
@@ -6,36 +6,26 @@ locale EdomArityAnalysis = ArityAnalysis +
   assumes Aexp_edom: "edom (Aexp e\<cdot>a) \<subseteq> fv e"
 begin
 
-lemma Aexp'_edom: "edom (Aexp' e\<cdot>a) \<subseteq> fv e"
-  by (cases a) (auto dest:set_mp[OF Aexp_edom])
+  lemma Aexp'_edom: "edom (Aexp' e\<cdot>a) \<subseteq> fv e"
+    by (cases a) (auto dest:set_mp[OF Aexp_edom])
+  
+  lemma Aexp_fresh_bot[simp]: assumes "atom v \<sharp> e" shows "(Aexp e\<cdot>a) v = \<bottom>"
+  proof-
+    from assms have "v \<notin> fv e" by (metis fv_not_fresh)
+    with Aexp_edom have "v \<notin> edom (Aexp e\<cdot>a)" by auto
+    thus ?thesis unfolding edom_def by simp
+  qed
+  
 
 end
 
-locale CorrectArityAnalysis = EdomArityAnalysis +
-  assumes Aexp_eqvt[eqvt]: "\<pi> \<bullet> Aexp = Aexp"
-  assumes Aexp_Var: "up \<cdot> n \<sqsubseteq> (Aexp (Var x) \<cdot> n) x"
-  assumes Aexp_subst_App_Lam: "Aexp (e[y::=x]) \<sqsubseteq> Aexp (App (Lam [y]. e) x)"
-  assumes Aexp_Lam: "Aexp (Lam [y]. e) \<cdot> n = env_delete y (Aexp e \<cdot>(pred\<cdot>n))"
-  assumes Aexp_App: "Aexp (App e x) \<cdot> n = Aexp e \<cdot>(inc\<cdot>n) \<squnion> AE_singleton x \<cdot> (up\<cdot>0)"
-  assumes Aexp_subst_restr: "x \<notin> S \<Longrightarrow> y \<notin> S \<Longrightarrow> (Aexp e[x::=y] \<cdot> a) f|` S = (Aexp e\<cdot>a) f|` S"
-
-locale CorrectArityAnalysis' = ArityAnalysis +
+locale CorrectArityAnalysis' = ArityAnalysis + EdomArityAnalysis +
   assumes Aexp[eqvt]: "\<pi> \<bullet> Aexp = Aexp"
   assumes Aexp_Var: "up \<cdot> n \<sqsubseteq> (Aexp (Var x)\<cdot>n) x"
   assumes Aexp_App: "Aexp e \<cdot>(inc\<cdot>n) \<squnion> AE_singleton x \<cdot> (up\<cdot>0) \<sqsubseteq>  Aexp (App e x) \<cdot> n"
-  assumes Aexp_subst_App_Lam: "Aexp (e[y::=x]) \<sqsubseteq> Aexp (App (Lam [y]. e) x)"
-  assumes Aexp_Lam: " env_delete y (Aexp e \<cdot>(pred\<cdot>n)) \<sqsubseteq> Aexp (Lam [y]. e) \<cdot> n"
+  assumes Aexp_Lam: "env_delete y (Aexp e \<cdot>(pred\<cdot>n)) \<sqsubseteq> Aexp (Lam [y]. e) \<cdot> n"
   assumes Aexp_subst: "Aexp (e[y::=x])\<cdot>a \<sqsubseteq> env_delete y ((Aexp e)\<cdot>a) \<squnion> AE_singleton x\<cdot>(up\<cdot>0)"
-
-locale CorrectArityAnalysisAheap = CorrectArityAnalysis + 
-  fixes Aheap :: "heap \<Rightarrow> AEnv \<rightarrow> AEnv"
-  assumes Aheap_eqvt[eqvt]: "\<pi> \<bullet> Aheap = Aheap"
-  assumes edom_Aheap: "edom (Aheap \<Gamma> \<cdot> ae) \<subseteq> domA \<Gamma>"
-  assumes Aheap_heap: "map_of \<Gamma> x = Some e' \<Longrightarrow> Aexp' e'\<cdot>((Aheap \<Gamma>\<cdot>ae) x) f|` domA \<Gamma> \<sqsubseteq> Aheap \<Gamma>\<cdot>ae"
-  assumes Aheap_heap3: "map_of \<Gamma> x = Some e' \<Longrightarrow> \<not> isLam e' \<Longrightarrow> (Aheap \<Gamma>\<cdot>ae) x = up\<cdot>0"
-  assumes Aheap_above_arg: "ae f|` domA \<Gamma> \<sqsubseteq> Aheap \<Gamma>\<cdot>ae"
-  assumes Aheap_subst: "x \<notin> domA \<Gamma> \<Longrightarrow> y \<notin> domA \<Gamma> \<Longrightarrow> Aheap \<Gamma>[x::h=y] = Aheap \<Gamma>"
-  assumes Aheap_cong: "ae f|` domA \<Gamma> = ae' f|` domA \<Gamma> \<Longrightarrow> Aheap \<Gamma>\<cdot>ae = Aheap \<Gamma>\<cdot>ae'"
+  assumes Aexp_subst_restr: "x \<notin> S \<Longrightarrow> y \<notin> S \<Longrightarrow> (Aexp e[x::=y] \<cdot> a) f|` S = (Aexp e\<cdot>a) f|` S"
 
 locale CorrectArityAnalysisAheap' = CorrectArityAnalysis' + 
   fixes Aheap :: "heap \<Rightarrow> exp \<Rightarrow> Arity \<rightarrow> AEnv"
@@ -43,32 +33,13 @@ locale CorrectArityAnalysisAheap' = CorrectArityAnalysis' +
   assumes edom_Aheap: "edom (Aheap \<Gamma> e\<cdot> a) \<subseteq> domA \<Gamma>"
   assumes Aheap_subst: "x \<notin> domA \<Gamma> \<Longrightarrow> y \<notin> domA \<Gamma> \<Longrightarrow> Aheap \<Gamma>[x::h=y] e[x ::=y]  = Aheap \<Gamma> e"
 
-locale CorrectArityAnalysisLet = CorrectArityAnalysisAheap +
-  assumes Aheap_heap2: "map_of \<Gamma> x = Some e' \<Longrightarrow> Aexp' e'\<cdot>((Aheap \<Gamma>\<cdot>(Aexp e\<cdot>a)) x) f|` (- domA \<Gamma>) \<sqsubseteq>  Aexp (Let \<Gamma> e)\<cdot>a"
-  assumes Aexp_Let_above: "Aexp e\<cdot>a f|` (- domA \<Gamma>) \<sqsubseteq> Aexp (Let \<Gamma> e)\<cdot>a"
-
 locale CorrectArityAnalysisLet' = CorrectArityAnalysisAheap' +
   assumes Aexp_Let: "ABinds \<Gamma>\<cdot>(Aheap \<Gamma> e\<cdot>a) \<squnion> Aexp e\<cdot>a \<sqsubseteq> Aheap \<Gamma> e\<cdot>a \<squnion>  Aexp (Let \<Gamma> e)\<cdot>a"
 
 locale CorrectArityAnalysisLetNoCard = CorrectArityAnalysisLet' +
   assumes Aheap_heap3: "x \<in> thunks \<Gamma> \<Longrightarrow> (Aheap \<Gamma> e\<cdot>a) x = up\<cdot>0"
  
-
-locale CorrectArityAnalysisCong = CorrectArityAnalysisAheap +
-  assumes Aexp_App_cong: "Aexp e\<cdot>(inc\<cdot>a) = Aexp e'\<cdot>(inc\<cdot>a) \<Longrightarrow> Aexp (App e x)\<cdot>a = Aexp (App e' x)\<cdot>a"
-  assumes Aexp_Lam_cong: "Aexp e\<cdot>(pred\<cdot>n) = Aexp e'\<cdot>(pred\<cdot>n) \<Longrightarrow> Aexp (Lam [y]. e) \<cdot> n = Aexp (Lam [y]. e') \<cdot> n"
-  assumes Aexp_Let_cong:
-    "domA \<Gamma> = domA \<Gamma>' \<Longrightarrow>
-     thunks \<Gamma> = thunks \<Gamma>' \<Longrightarrow>
-     (\<And> x a. x \<in> domA \<Gamma> \<Longrightarrow> up\<cdot>a \<sqsubseteq> (Aheap \<Gamma>'\<cdot>(Aexp e\<cdot>a)) x \<Longrightarrow> Aexp (the (map_of \<Gamma> x))\<cdot>a = Aexp (the (map_of \<Gamma>' x))\<cdot>a) \<Longrightarrow>
-     Aexp e\<cdot>a = Aexp e'\<cdot>a \<Longrightarrow>
-     Aexp (Let \<Gamma> e)\<cdot>a = Aexp (Let \<Gamma>' e')\<cdot>a"
-  assumes Aheap_cong2: "domA \<Gamma> = domA \<Gamma>' \<Longrightarrow>
-    (\<And> x a. x \<in> domA \<Gamma> \<Longrightarrow> up\<cdot>a \<sqsubseteq> (Aheap \<Gamma>'\<cdot>ae) x \<Longrightarrow> Aexp (the (map_of \<Gamma> x))\<cdot>a = Aexp (the (map_of \<Gamma>' x))\<cdot>a) \<Longrightarrow>
-    Aheap \<Gamma>\<cdot>ae = Aheap \<Gamma>'\<cdot>ae"
-
-
-context CorrectArityAnalysis
+context CorrectArityAnalysis'
 begin
 
 lemma Aexp_Var_singleton: "AE_singleton x \<cdot> (up\<cdot>n) \<sqsubseteq> Aexp (Var x) \<cdot> n"
