Launchbury/RedsImprovesArityAnalysis.thy
@@ -119,12 +119,15 @@ case (Application y \<Gamma> e x L \<Delta> \<Theta> z e' ae n)
     note IH1 = env_restr_below_subset[OF subset2 Application(3)[OF prem3, where n = "inc\<^sub>\<bottom>\<cdot>n"], unfolded up Aexp'_simps inc_bot_simps] 
     note IH2 = env_restr_below_subset[OF subset1 Application(5)[OF prem1, where n = n], unfolded up Aexp'_simps]
     have "Afix \<Theta>\<cdot>(Aexp z\<cdot>n' \<squnion> ae)  f|` ?S  \<sqsubseteq> Afix \<Delta>\<cdot>(Aexp e'[y::=x]\<cdot>n' \<squnion> ae)  f|` ?S" by (rule IH2)
-    also have "\<dots> \<sqsubseteq> Afix \<Delta>\<cdot>(Aexp (App (Lam [y]. e') x)\<cdot>n' \<squnion> ae) f|` ?S" by (intro monofun_cfun_arg monofun_cfun_fun env_restr_mono Aexp_subst_App_Lam join_mono below_refl)
-    also have "\<dots> = Afix \<Delta>\<cdot>(Aexp (Lam [y]. e')\<cdot>(inc\<cdot>n') \<squnion> AE_singleton x \<cdot> (up\<cdot>0) \<squnion> ae)  f|` ?S"  by (rule arg_cong[OF Aexp_App])
-    also have "\<dots> = Afix \<Delta>\<cdot>(Aexp (Lam [y]. e')\<cdot>(inc\<cdot>n') \<squnion> (AE_singleton x\<cdot>(up\<cdot>0) \<squnion> ae))  f|` ?S"  by simp
+    also have "\<dots> \<sqsubseteq> Afix \<Delta>\<cdot>(env_delete y (Aexp e'\<cdot>n') \<squnion>  AE_singleton x \<cdot> (up\<cdot>0) \<squnion> ae)  f|` ?S"
+      by (intro monofun_cfun_arg monofun_cfun_fun env_restr_mono Aexp_subst join_mono below_refl)  
+    also have "\<dots> = Afix \<Delta>\<cdot>(env_delete y (Aexp e'\<cdot>(pred\<cdot>(inc\<cdot>n'))) \<squnion> (AE_singleton x \<cdot> (up\<cdot>0) \<squnion> ae))  f|` ?S" by simp
+    also have "\<dots> \<sqsubseteq> Afix \<Delta>\<cdot>(Aexp (Lam [y]. e')\<cdot>(inc\<cdot>n') \<squnion> (AE_singleton x \<cdot> (up\<cdot>0) \<squnion> ae))  f|` ?S"
+      by (intro monofun_cfun_arg monofun_cfun_fun env_restr_mono Aexp_Lam join_mono below_refl)  
     also have "\<dots> \<sqsubseteq> Afix \<Gamma>\<cdot>(Aexp e\<cdot>(inc\<cdot>n') \<squnion> (AE_singleton x\<cdot>(up\<cdot>0) \<squnion> ae)) f|` ?S" by (rule IH1)
     also have "\<dots> = Afix \<Gamma>\<cdot>(Aexp e\<cdot>(inc\<cdot>n') \<squnion> AE_singleton x\<cdot>(up\<cdot>0) \<squnion> ae)  f|` ?S" by simp
-    also have "\<dots> = Afix \<Gamma>\<cdot>(Aexp (App e x)\<cdot>n' \<squnion> ae)  f|` ?S" by (rule arg_cong[OF Aexp_App[symmetric]])
+    also have "\<dots> \<sqsubseteq> Afix \<Gamma>\<cdot>(Aexp (App e x)\<cdot>n' \<squnion> ae)  f|` ?S" 
+      by (intro monofun_cfun_arg monofun_cfun_fun env_restr_mono Aexp_App join_mono below_refl)  
     finally
     show ?thesis unfolding up by simp
   qed
